src/ident.v
@@ -1,0 +1,183 @@
+From Coq Require Import FMapAVL.
+From Coq Require Import String.
+Require Import OrderedType.
+Require Import Coq.Structures.OrdersEx.
+
+Inductive ident :=
+    | Id_s : string -> ident
+    | Num : nat -> ident.
+Scheme Equality for ident.
+
+Lemma ident_beq_eq: forall x y, ident_beq x y = true <-> x = y.
+Proof.
+    intros; split; intro.
+    + apply internal_ident_dec_bl; assumption.
+    + apply internal_ident_dec_lb; assumption.
+Qed.
+
+Module Ident_as_OT_map <: OrderedType.
+    Definition t := ident.
+    (* Include HasUsualEq <+ UsualIsEq. *)
+    Definition eq := @eq t.
+    Definition eqb := ident_beq.
+    Definition eqb_eq := ident_beq_eq.
+    Definition eq_dec := ident_eq_dec.
+    (* Include HasEqBool2Dec. *)
+
+    Definition eq_refl := @eq_refl t.
+    Definition eq_sym := @eq_sym t.
+    Definition eq_trans := @eq_trans t.
+
+    Definition cmp (a b : ident)
+        := match a, b with
+            | Id_s a, Id_s b => String_as_OT.compare a b
+            | Id_s _, Num _ => Lt
+            | Num _, Id_s _ => Gt
+            | Num a, Num b => Nat.compare a b
+        end.
+
+    Definition lt (a b : ident) := cmp a b = Lt.
+
+    #[global]
+    Instance lt_compat : Proper (eq==>eq==>iff) lt.
+    Proof.
+        intros x x' H; destruct H.
+        intros y y' H; destruct H.
+        split; trivial.
+    Qed.
+
+    Lemma compare : forall x y, Compare lt eq x y.
+    Proof.
+        intros x y.
+        pose (p := cmp x y).
+        destruct x as [s1|n1]; destruct y as [s2|n2]; simpl in *.
+        1: pose (p' := String_as_OT.compare_spec s1 s2); generalize p'; clear p'; fold p.
+        4: pose (p' := Nat_as_OT.compare_spec n1 n2); generalize p'; clear p'; fold p.
+        all: case_eq p; unfold p; clear p.
+        4,6,7,8: discriminate.
+        all: intro H.
+        1-3: intro H2; [> constructor 2 | constructor 1 | constructor 3].
+        6-8: intro H2; [> constructor 2 | constructor 1 | constructor 3].
+        4-5: [> constructor 1 | constructor 3].
+        all: unfold lt, eq; simpl; auto.
+        1,3: f_equal.
+        all: inversion H2; auto.
+        rewrite PeanoNat.Nat.compare_lt_iff; assumption.
+    Qed.
+
+    #[global]
+    Instance lt_strorder : StrictOrder lt.
+    Proof.
+        destruct (String_as_OT.lt_strorder).
+        destruct (Nat_as_OT.lt_strorder).
+        split.
+        {
+            unfold Irreflexive, Reflexive, complement, lt in *.
+            intro x; destruct x as [s|n]; simpl.
+            + apply StrictOrder_Irreflexive.
+            + rewrite PeanoNat.Nat.compare_lt_iff; apply StrictOrder_Irreflexive0.
+        }
+        {
+            unfold Transitive, lt in *.
+            intro x; destruct x as [s1|n1]; simpl.
+            all: intro x; destruct x as [s2|n2]; simpl.
+            all: intro x; destruct x as [s3|n3]; simpl; trivial.
+            + apply StrictOrder_Transitive.
+            + discriminate.
+            + discriminate.
+            + do 3 rewrite PeanoNat.Nat.compare_lt_iff;
+                apply StrictOrder_Transitive0.
+        }
+    Qed.
+
+    Definition lt_trans := StrictOrder_Transitive.
+    Lemma lt_not_eq : forall x y, lt x y -> x <> y.
+    Proof.
+        pose (p := StrictOrder_Irreflexive).
+        unfold Irreflexive, Reflexive, complement in *.
+        intros x y Hlt HEq; destruct HEq; apply p in Hlt.
+        assumption.
+    Qed.
+
+End Ident_as_OT_map.
+
+Module imap := Make Ident_as_OT_map.
+
+From Coq Require Import MSets.
+
+Module Ident_as_OT_set <: UsualOrderedType.
+    Definition t := ident.
+    Include HasUsualEq <+ UsualIsEq.
+    Definition eqb := ident_beq.
+    Definition eqb_eq := ident_beq_eq.
+    Include HasEqBool2Dec.
+
+    Definition compare (a b : ident)
+        := match a, b with
+            | Id_s a, Id_s b => String_as_OT.compare a b
+            | Id_s _, Num _ => Lt
+            | Num _, Id_s _ => Gt
+            | Num a, Num b => Nat.compare a b
+        end.
+
+    Definition lt (a b : ident) := compare a b = Lt.
+
+#[global]
+    Instance lt_compat : Proper (eq==>eq==>iff) lt.
+    Proof.
+        intros x x' H; destruct H.
+        intros y y' H; destruct H.
+        split; trivial.
+    Qed.
+
+    Lemma compare_spec : forall x y, CompSpec eq lt x y (compare x y).
+    Proof.
+        intros x y.
+        unfold CompSpec.
+        destruct x as [s1|n1]; destruct y as [s2|n2]; simpl.
+        all: unfold lt, eq; simpl.
+        2,3: constructor; reflexivity.
+        {
+            pose (p := String_as_OT.compare_spec s1 s2).
+            unfold CompSpec, String_as_OT.eq, String_as_OT.lt in p.
+            generalize p; clear p; intro p.
+            destruct (String_as_OT.compare s1 s2); inversion p; constructor; auto.
+            f_equal; assumption.
+        }
+        {
+            pose (p := Nat_as_OT.compare_spec n1 n2).
+            unfold CompSpec, Nat_as_OT.eq, Nat_as_OT.lt in p.
+            generalize p; clear p; intro p.
+            destruct (Nat_as_OT.compare n1 n2); inversion p; constructor; auto.
+            rewrite PeanoNat.Nat.compare_lt_iff; assumption.
+        }
+    Qed.
+
+#[global]
+    Instance lt_strorder : StrictOrder lt.
+    Proof.
+        destruct (String_as_OT.lt_strorder).
+        destruct (Nat_as_OT.lt_strorder).
+        split.
+        {
+            unfold Irreflexive, Reflexive, complement, lt in *.
+            intro x; destruct x as [s|n]; simpl.
+            + apply StrictOrder_Irreflexive.
+            + rewrite PeanoNat.Nat.compare_lt_iff; apply StrictOrder_Irreflexive0.
+        }
+        {
+            unfold Transitive, lt in *.
+            intro x; destruct x as [s1|n1]; simpl.
+            all: intro x; destruct x as [s2|n2]; simpl.
+            all: intro x; destruct x as [s3|n3]; simpl; trivial.
+            + apply StrictOrder_Transitive.
+            + discriminate.
+            + discriminate.
+            + do 3 rewrite PeanoNat.Nat.compare_lt_iff;
+                apply StrictOrder_Transitive0.
+        }
+    Qed.
+
+End Ident_as_OT_set.
+
+Module iset := Make Ident_as_OT_set.
