src/normalization/collectProof.v
@@ -1,6 +1,6 @@
-From Usuba Require Import usuba_AST collect usuba_sem equiv_rel.
-From Coq Require Import MSets MSets.MSetToFiniteSet MSets.MSetFacts.
-Require Import Coq.Structures.OrdersEx.
+From Usuba Require Import ident usuba_AST collect usuba_sem equiv_rel.
+(* From Coq Require Import MSets MSets.MSetToFiniteSet MSets.MSetFacts. *)
+(* Require Import Coq.Structures.OrdersEx. *)
 From mathcomp Require Import all_ssreflect.
 Require Import Coq.Sets.Ensembles.
 
